Well-formedness for terms & contexts (#33)
* Specify well-formed terms

* Hole well-formedness

* Context well-formedness

* Prove crucial lemma on well-formedness of filled holes

theories/Context.v
@@ -27,6 +27,24 @@ Fixpoint fv_ctx ctx : set string :=
 
 Instance fv_context : FV context := { fv := fv_ctx; }.
 
+Inductive WFContext : context -> Prop :=
+  | WFCtxEmpty :
+      WFContext CtxEmpty
+  | WFCtxHasTy : forall x t,
+      WFContext (CtxHasTy x t)
+  | WFCtxComma : forall g g',
+      WFContext g ->
+      WFContext g' ->
+      DisjointSets (fv g) (fv g') ->
+      WFContext (CtxComma g g')
+  | WFCtxSemic : forall g g',
+      WFContext g ->
+      WFContext g' ->
+      DisjointSets (fv g) (fv g') ->
+      WFContext (CtxSemic g g')
+  .
+Hint Constructors WFContext : core.
+
 (* Argument order matches notation: (CtxLEq G G') === (G <= G') *)
 Inductive CtxLEq (G G' : context) : Prop :=
   (* TODO *)
