theories/Hole.v
@@ -76,3 +76,111 @@ Lemma fv_fill : forall h plug ctx,
   SetEq (fv ctx) (set_union (fv plug) (fv h)).
 Proof. intros. induction H; sfirstorder. Qed.
 Hint Resolve fv_fill : core.
+
+Inductive WFHole : hole -> Prop :=
+  | WFHoleHere :
+      WFHole HoleHere
+  | WFHoleCommaL : forall lhs rhs,
+      WFHole lhs ->
+      WFContext rhs ->
+      DisjointSets (fv lhs) (fv rhs) ->
+      WFHole (HoleCommaL lhs rhs)
+  | WFHoleCommaR : forall lhs rhs,
+      WFContext lhs ->
+      WFHole rhs ->
+      DisjointSets (fv lhs) (fv rhs) ->
+      WFHole (HoleCommaR lhs rhs)
+  | WFHoleSemicL : forall lhs rhs,
+      WFHole lhs ->
+      WFContext rhs ->
+      DisjointSets (fv lhs) (fv rhs) ->
+      WFHole (HoleSemicL lhs rhs)
+  | WFHoleSemicR : forall lhs rhs,
+      WFContext lhs ->
+      WFHole rhs ->
+      DisjointSets (fv lhs) (fv rhs) ->
+      WFHole (HoleSemicR lhs rhs)
+  .
+Hint Constructors WFHole : core.
+
+Theorem wf_ctx_plug : forall GD,
+  WFContext GD ->
+  forall G D,
+  Fill G D GD ->
+  WFContext D.
+Proof.
+  intros GD Hc G D Hf. generalize dependent Hc.
+  induction Hf; intros; try (apply IHHf; sinvert Hc); assumption.
+Qed.
+Hint Resolve wf_ctx_plug : core.
+
+Theorem fill_disjoint_l : forall G D GD (s : context),
+  Fill G D GD ->
+  DisjointSets (fv GD) (fv s) ->
+  DisjointSets (fv G) (fv s).
+Proof.
+  cbn in *. intros G D GDG s Hf Hd. split; intros H C; specialize (Hd x) as [Hlr Hrl];
+  (apply Hrl; [| eapply fv_fill; [| right]]; eassumption).
+Qed.
+Hint Resolve fill_disjoint_l : core.
+
+Theorem fill_disjoint_r : forall G D GD (s : context),
+  Fill G D GD ->
+  DisjointSets (fv s) (fv GD) ->
+  DisjointSets (fv s) (fv G).
+Proof.
+  cbn in *. intros G D GDG s Hf Hd. split; intros H C; specialize (Hd x) as [Hlr Hrl];
+  (apply Hlr; [| eapply fv_fill; [| right]]; eassumption).
+Qed.
+Hint Resolve fill_disjoint_r : core.
+
+Theorem wf_ctx_hole : forall GD,
+  WFContext GD ->
+  forall G D,
+  Fill G D GD ->
+  WFHole G.
+Proof.
+  intros GD Hc G D Hf. generalize dependent Hc.
+  induction Hf; intros; [constructor | | | |]; sinvert Hc; constructor; try apply IHHf; try assumption;
+  try (eapply fill_disjoint_l; eassumption); eapply fill_disjoint_r; eassumption.
+Qed.
+Hint Resolve wf_ctx_hole : core.
+
+Lemma wf_fill : forall G D GD,
+  Fill G D GD ->
+  WFHole G ->
+  WFContext D ->
+  DisjointSets (fv G) (fv D) ->
+  WFContext GD.
+Proof.
+  intros G D GD Hf HG HD Hd. generalize dependent D. generalize dependent GD.
+  induction HG; cbn in *; intros; sinvert Hf; [assumption | | | |];
+  constructor; try assumption (* 1/3 *); try eapply IHHG; clear IHHG; try eassumption;
+  apply fv_fill in H5; (* <-- this is the crucial move! *) sfirstorder.
+Qed.
+Hint Resolve wf_fill : core.
+
+Lemma fill_wf_disjoint : forall G D GD,
+  Fill G D GD ->
+  WFContext GD ->
+  DisjointSets (fv G) (fv D).
+Proof.
+  intros G D GD Hf Hwf.
+  cbn in *. intro x. assert (Hiff := fv_fill _ _ _ Hf x). cbn in Hiff.
+  generalize dependent D. generalize dependent GD. induction G; cbn in *; intros; [sfirstorder | | | |];
+  sinvert Hf; sinvert Hwf; assert (Hfv := fv_fill _ _ _ H3); cbn in *; specialize (H4 x) as [Hlr Hrl];
+  (edestruct IHG as [IH1 IH2]; [| eassumption | apply fv_fill |]; [assumption | assumption |]; sfirstorder).
+Qed.
+Hint Resolve fill_wf_disjoint : core.
+
+Theorem wf_hole_iff : forall G D GD,
+  Fill G D GD -> (
+    WFContext GD <-> (
+      WFHole G /\
+      WFContext D /\
+      DisjointSets (fv G) (fv D))). (* <-- this should fix the above comment *)
+Proof.
+  intros G D GD Hf. split; [intro Hwf | intros [HG [HD Hd]]].
+  - split; [| split]; [eapply wf_ctx_hole | eapply wf_ctx_plug | eapply fill_wf_disjoint]; eassumption.
+  - eapply wf_fill; eassumption.
+Qed.
