theories/Typing.v
@@ -1,7 +1,10 @@
+From Coq Require Import String.
+From Hammer Require Import Tactics.
 From LambdaST Require Import
   Context
   FV
   Hole
+  Sets
   Terms
   Types.
 
@@ -14,7 +17,7 @@ Inductive Typed : context -> term -> type -> Prop :=
       G |- e1 \in s ->
       G |- e2 \in t ->
       G |- (e1, e2) \in TyPar s t
-  | T_Par_L : forall G x y z s t e r Gxsyt Gzst,
+  | TParL : forall G x y z s t e r Gxsyt Gzst,
       x <> y ->
       ~fv G x ->
       ~fv G y ->
@@ -29,8 +32,9 @@ Inductive Typed : context -> term -> type -> Prop :=
   | TCatR : forall G D e1 e2 s t,
       G |- e1 \in s ->
       D |- e2 \in t ->
+      DisjointSets (fv G) (fv D) ->
       CtxSemic G D |- (e1; e2) \in TyDot s t
-  | T_Cat_L : forall G x y z s t e r Gxsyt Gzst,
+  | TCatL : forall G x y z s t e r Gxsyt Gzst,
       x <> y ->
       ~fv G x ->
       ~fv G y ->
@@ -54,7 +58,7 @@ Inductive Typed : context -> term -> type -> Prop :=
       CtxLEq G G' ->
       G' |- e \in s ->
       G |- e \in s
-  | T_Let : forall G D x e e' s t Gxs GD,
+  | TLet : forall G D x e e' s t Gxs GD,
       ~fv G x ->
       D |- e \in s ->
       (*
@@ -65,7 +69,7 @@ Inductive Typed : context -> term -> type -> Prop :=
       Fill G D GD ->
       Gxs |- e' \in t ->
       GD |- TmLet x e e' \in t
-  | T_Drop : forall G x s t e Ge Gxs,
+  | TDrop : forall G x s t e Ge Gxs,
       (*
       fill G CtxEmpty |- e \in t ->
       fill G (CtxHasTy x s) |- TmDrop x e \in t
@@ -77,8 +81,51 @@ Inductive Typed : context -> term -> type -> Prop :=
 where "G '|-' x '\in' T" := (Typed G x T).
 Hint Constructors Typed : core.
 
-(* TODO:
+Theorem typed_fv : forall G e s,
+  G |- e \in s ->
+  forall x,
+  fv e x ->
+  fv G x.
+Proof.
+  intros G e s Ht x Hfv. generalize dependent x. (* just for naming *)
+  induction Ht; try rename x into x' (* hands off my `x`! *); intros x H'; cbn in *.
+  - destruct H'; [apply IHHt1 | apply IHHt2]; assumption.
+  - eapply fv_fill. { eassumption. } cbn. destruct H' as [| [[H2' H3'] H4]]; [left | right]. { assumption. }
+    specialize (IHHt _ H2'). eapply fv_fill in IHHt; [| eassumption].
+    cbn in IHHt. destruct IHHt; [| assumption]. destruct H5; contradiction H5.
+  - destruct H'; [left; apply IHHt1 | right; apply IHHt2]; assumption.
+  - eapply fv_fill. { eassumption. } cbn. destruct H' as [| [[H2' H3'] H4]]; [left | right]. { assumption. }
+    specialize (IHHt _ H2'). eapply fv_fill in IHHt; [| eassumption].
+    cbn in IHHt. destruct IHHt; [| assumption]. destruct H5; contradiction H5.
+  - destruct H' as [].
+  - destruct H' as [].
+  - eapply fv_fill. { eassumption. } cbn. left. assumption.
+  - cbn in *. specialize (IHHt _ H'). invert H. (* TODO: SubCtx hasn't been defined yet, so holds vacuously *)
+  - eapply fv_fill. { eassumption. } cbn. destruct H' as [H' | [H' H'']]; [left | right]. { apply IHHt1. assumption. }
+    specialize (IHHt2 _ H'). eapply fv_fill in IHHt2; [| eassumption].
+    cbn in IHHt2. destruct IHHt2. { contradiction. } assumption.
+  - eapply fv_fill. { eassumption. } cbn. destruct H'. specialize (IHHt _ H1).
+    eapply fv_fill in IHHt as [IH | IH]; [| | eassumption]. { destruct IH. } right. assumption.
+Qed.
+Hint Resolve typed_fv : core.
+
+(* TODO: add WF weakening theorem assuming all FVs are covered, then use the above to prove the below *)
+
 Theorem typed_wf_term : forall G x T,
   G |- x \in T ->
   WFTerm (fv G) x.
-*)
+Proof.
+  intros. induction H; intros.
+  - (* (e1, e2) *)
+    constructor; assumption.
+  - (* let (x, y) = z in e *)
+    shelve. (* until `inert` (might change something) *)
+    (*
+    constructor; cbn in *.
+    + assert (Fxsyt := fv_fill _ _ _ H2). assert (Fzst := fv_fill _ _ _ H3). cbn in *.
+      eapply wf_set_eq; [| eassumption]. cbn. intro test. rewrite Fzst. rewrite Fxsyt. split; intros H'.
+      * destruct H' as [H' | H']. { right. assumption. } left. split. { right. assumption. } intro. subst. Search test. best use: fv_fill time: 10.
+        destruct H' as [H' | H']; subst. { right. left. reflexivity. } right. right. best.
+    *)
+  - (* (e1; e2) *)
+    cbn in *. constructor. eapply typed_fv in H. Abort. (* TODO *)
